% !Mode:: "TeX:UTF-8"
\chapter{矢量分析公式}\label{vector}

\section{求和约定}
矢量：
\begin{equation}
\symbfit{a} = a^i \symbf{e}_i = \sum_{i=1}^{3} a^i \symbf{e}_i
\end{equation}

二阶张量：
\begin{equation}
\symbfit{\sigma} = \sigma^{ij} \symbf{e}_i \symbf{e}_j = \sum_{i=1}^{3}\sum_{j=1}^{3}  \sigma^{ij} \symbf{e}_i \symbf{e}_j
\end{equation}

\section{代数运算}
数量积：
\begin{equation}
\symbf{e}_i \cdot\symbf{e}_j = \delta_{ij} =
    \begin{cases}
    1 & i=j \\
    0 & i\neq j
    \end{cases}
\end{equation}
%
\begin{equation}
\symbfit{a} \cdot \symbfit{b}
=
a^i \symbf{e}_i \cdot b^j \symbf{e}_j
=
a^i b^j \symbf{e}_i \cdot\symbf{e}_j
= a^i b^j \delta_{ij}
= a^i b^i
\end{equation}

矢量积：
\begin{equation}
\symbf{e}_i \times\symbf{e}_j = \varepsilon_{ijk}\symbf{e}_k =
    \begin{cases}
    1 & ijk=123\text{或}231\text{或}312 \\
    -1 & ijk=321\text{或}213\text{或}132 \\
    0 & ijk\text{其他}
    \end{cases}
\end{equation}
%
\begin{equation}
\symbfit{a} \times \symbfit{b}
=
a^i \symbf{e}_i \times b^j \symbf{e}_j
=
a^i b^j  \varepsilon_{ijk}\symbf{e}_k
\end{equation}
%
\begin{equation}
\varepsilon_{ijk} \varepsilon_{ilm} =
\delta_{jl}\delta_{km} - \delta_{jm}\delta_{kl}
\end{equation}
%
\section{恒等式}
%
\begin{equation}
\left( \symbfit{a} \times \symbfit{b} \right) \cdot \symbfit{c}
=
\left( \symbfit{b} \times \symbfit{c} \right) \cdot \symbfit{a}
=
\left( \symbfit{c} \times \symbfit{a} \right) \cdot \symbfit{b}
\end{equation}
%
\begin{equation}
\left( \symbfit{a} \times \symbfit{b} \right) \times \symbfit{c}
=
\left( \symbfit{a} \cdot \symbfit{c} \right)  \symbfit{b}
-
\left( \symbfit{b} \cdot \symbfit{c} \right)  \symbfit{a}
\end{equation}
%
\begin{equation}
\nabla \times \left( \nabla \phi \right)
=
\symbf{0}
\end{equation}
%
\begin{equation}
\nabla \cdot \left( \nabla \times \phi \right)
=
0
\end{equation}
%
\begin{equation}
\nabla \cdot \left( \phi \symbfit{a} \right)
=
\phi \left( \nabla \cdot \symbfit{a} \right)
+
\nabla \phi \cdot \symbfit{a}
\end{equation}
%
\begin{equation}
\nabla \times \left( \phi \symbfit{a} \right)
=
\phi \left( \nabla \times \symbfit{a} \right)
+
\nabla \phi \times \symbfit{a}
\end{equation}
%
\begin{equation}
\nabla \cdot \left( \symbfit{a} \times \symbfit{b} \right)
=
\left( \nabla \times \symbfit{a} \right) \cdot \symbfit{b}
-
\symbfit{a} \cdot  \left( \nabla \times \symbfit{b} \right)
\end{equation}
%
\begin{equation}
\nabla \times \left( \symbfit{a} \times \symbfit{b} \right)
=
\left( \symbfit{b} \cdot \nabla \right) \symbfit{a}
-
\left( \symbfit{a} \cdot \nabla \right) \symbfit{b}
+
\symbfit{a} \left( \nabla \cdot \symbfit{b} \right)
-
\symbfit{b} \left( \nabla \cdot \symbfit{a} \right)
\end{equation}
%
\begin{equation}
\nabla \left( \symbfit{a} \cdot \symbfit{b} \right)
=
\symbfit{a} \times \left( \nabla \times \symbfit{b} \right)
+
\symbfit{b} \times \left( \nabla \times \symbfit{a} \right)
+
\left( \symbfit{a} \cdot \nabla \right) \symbfit{b}
+
\left( \symbfit{b} \cdot \nabla \right) \symbfit{a}
\end{equation}
%
\begin{equation}
\nabla \times \left( \nabla \times \symbfit{a} \right)
=
\nabla \left( \nabla \cdot \symbfit{a} \right)
-
\nabla^2 \symbfit{a}
\end{equation}
%
\begin{equation}\label{}
\left( \symbfit{a} \cdot \nabla \right) \symbfit{a}
=
\left( \nabla \times \symbfit{a} \right) \times \symbfit{a}
+
\nabla \left( \frac{1}{2} a^2 \right)
\end{equation}
%
